x86/OrderedLinking.v
@@ -373,20 +373,6 @@ Global Opaque Linker_prog_ordered.
 
 
 
-(** matching modulo the permutation of definitions *)
-
-Definition match_prog {F V} (p tp: program F V) :=
-  Permutation (prog_defs p) (prog_defs tp) 
-  /\ prog_main p = prog_main tp
-  /\ prog_public p = prog_public tp.
-
-Lemma transf_program_match:
-  forall F V (p: program F V), match_prog p p.
-Proof.
-  intros. red. 
-  repeat (split; auto).
-Qed.
-
 Lemma PTree_extract_elements_pres_get : forall A id ids defs (t t':PTree.t A),
     ~In id ids ->
     PTree_extract_elements ids t = Some (defs, t') ->
@@ -657,52 +643,3 @@ Proof.
   rewrite <- PUB1. auto.
   rewrite <- PUB2. auto.
 Qed.
-
-
-(** Commutativity between permutation and linking *)
-Instance TransfPermuteOrderedLink1 {F V} {LV: Linker V}
-  : @TransfLink _ _ (Linker_prog (fundef F) V) (Linker_prog_ordered F V) match_prog.
-Proof.
-  Local Transparent Linker_prog.
-  red. unfold match_prog. cbn. 
-  intros until p.
-  intros LINK (PERM1 & MAINEQ1 & PUBEQ1) (PERM2 & MAINEQ2 & PUBEQ2).
-  generalize LINK. intros LINK'.
-  unfold link_prog in LINK.
-  destr_in LINK. inv LINK. cbn.
-  repeat (rewrite andb_true_iff in Heqb). 
-  destruct Heqb as (((MAINEQ & NORPT1) & NORPT2) & CHECK).
-  destruct ident_eq; try discriminate.
-  destruct list_norepet_dec; try discriminate.
-  destruct list_norepet_dec; try discriminate.
-  unfold link_prog_ordered.
-  assert (prog_main tp1 = prog_main tp2) as MAINEQ3 by congruence.
-  rewrite MAINEQ3.
-  destruct ident_eq; try congruence. cbn.
-  assert (list_norepet (map fst (prog_defs tp1))) as NORPT3.
-  { eapply Permutation_list_norepet_map; eauto. }
-  destruct list_norepet_dec; try contradiction. cbn.
-  assert (list_norepet (map fst (prog_defs tp2))) as NORPT4.
-  { eapply Permutation_list_norepet_map; eauto. }
-  destruct list_norepet_dec; try contradiction. cbn.  
-  edestruct (@extract_defs_exists F V _ tp1 tp2) as (defs1 & t1 & EXTR); eauto.
-  eapply prog_linkable_permutation; eauto.
-  rewrite EXTR. 
-  eexists; split; eauto.
-  cbn.
-  repeat (split; auto).
-  generalize (PTree_extract_elements_permutation _ _ _ _ EXTR).
-  intros PERM3. 
-  apply Permutation_trans with (defs1 ++ PTree.elements t1).
-  eapply Permutation_trans; [| exact PERM3].
-  unfold prog_option_defmap.
-  eapply PTree_combine_permutation; eauto.
-  apply Permutation_app_comm.
-  congruence.
-  congruence.
-Qed.
-
-Instance TransfPermuteOrderedLink2 {F V} {LV: Linker V}
-  : @TransfLink _ _ (Linker_prog_ordered F V) (Linker_prog (fundef F) V) match_prog.
-Proof.
-Admitted.
