x86/PermuteProgproof.v
@@ -5,11 +5,24 @@
 
 (** * Preservation of semantics under the permutation of definitions for RealAsm *)
 Require Import Coqlib Errors.
-Require Import Integers Floats AST Linking OrderedLinking.
+Require Import Integers Floats AST.
 Require Import Values Memory Events Globalenvs Smallstep.
 Require Import Permutation.
 Require Import Asm RealAsm.
 
+(** matching modulo the permutation of definitions *)
+
+Definition match_prog {F V} (p tp: AST.program F V) :=
+  Permutation (prog_defs p) (prog_defs tp) 
+  /\ prog_main p = prog_main tp
+  /\ prog_public p = prog_public tp.
+
+Lemma transf_program_match:
+  forall F V (p: AST.program F V), match_prog p p.
+Proof.
+  intros. red. 
+  repeat (split; auto).
+Qed.
 
 (** Preservation of semantics under permutation *)
 Section PRESERVATION.
