x86/PermuteProgSep.v
@@ -1,0 +1,61 @@
+(* *******************  *)
+(* Author: Yuting Wang  *)
+(* Date:   Dec 12th, 2019 *)
+(* *******************  *)
+
+(** * Separate compilation for permutation of definitions *)
+Require Import Coqlib Errors Maps.
+Require Import Integers Floats AST.
+Require Import Values Memory Events Linking OrderedLinking.
+Require Import Permutation.
+Require Import PermuteProgproof.
+
+Local Transparent Linker_prog_ordered.
+
+(** Commutativity between permutation and linking *)
+Instance TransfPermuteOrderedLink1 {F V} {LV: Linker V}
+  : @TransfLink _ _ (Linker_prog (fundef F) V) (Linker_prog_ordered F V) match_prog.
+Proof.
+  Local Transparent Linker_prog.
+  red. unfold match_prog. cbn. 
+  intros until p.
+  intros LINK (PERM1 & MAINEQ1 & PUBEQ1) (PERM2 & MAINEQ2 & PUBEQ2).
+  generalize LINK. intros LINK'.
+  unfold link_prog in LINK.
+  destr_in LINK. inv LINK. cbn.
+  repeat (rewrite andb_true_iff in Heqb). 
+  destruct Heqb as (((MAINEQ & NORPT1) & NORPT2) & CHECK).
+  destruct ident_eq; try discriminate.
+  destruct list_norepet_dec; try discriminate.
+  destruct list_norepet_dec; try discriminate.
+  unfold link_prog_ordered.
+  assert (prog_main tp1 = prog_main tp2) as MAINEQ3 by congruence.
+  rewrite MAINEQ3.
+  destruct ident_eq; try congruence. cbn.
+  assert (list_norepet (map fst (prog_defs tp1))) as NORPT3.
+  { eapply Permutation_list_norepet_map; eauto. }
+  destruct list_norepet_dec; try contradiction. cbn.
+  assert (list_norepet (map fst (prog_defs tp2))) as NORPT4.
+  { eapply Permutation_list_norepet_map; eauto. }
+  destruct list_norepet_dec; try contradiction. cbn.  
+  edestruct (@extract_defs_exists F V _ tp1 tp2) as (defs1 & t1 & EXTR); eauto.
+  eapply prog_linkable_permutation; eauto.
+  rewrite EXTR. 
+  eexists; split; eauto.
+  cbn.
+  repeat (split; auto).
+  generalize (PTree_extract_elements_permutation _ _ _ _ EXTR).
+  intros PERM3. 
+  apply Permutation_trans with (defs1 ++ PTree.elements t1).
+  eapply Permutation_trans; [| exact PERM3].
+  unfold prog_option_defmap.
+  eapply PTree_combine_permutation; eauto.
+  apply Permutation_app_comm.
+  congruence.
+  congruence.
+Qed.
+
+Instance TransfPermuteOrderedLink2 {F V} {LV: Linker V}
+  : @TransfLink _ _ (Linker_prog_ordered F V) (Linker_prog (fundef F) V) match_prog.
+Proof.
+Admitted.
