x86/RelocProgSyneq.v
@@ -14,6 +14,14 @@ Definition symbtable_syneq (s1 s2: symbtable) : Prop :=
   Permutation (PTree.elements (symbtable_to_tree s1))
               (PTree.elements (symbtable_to_tree s2)).
 
+Lemma symbtable_syneq_refl: forall t,
+    symbtable_syneq t t.
+Proof.
+  unfold symbtable_syneq.
+  intros. 
+  apply Permutation_refl; eauto.
+Qed.
+
 Lemma symbtable_syneq_symm: forall t1 t2,
     symbtable_syneq t1 t2 -> symbtable_syneq t2 t1.
 Proof.
@@ -41,3 +49,38 @@ Definition reloc_prog_syneq (p tp: program) : Prop :=
   /\ prog_strtable p = prog_strtable tp
   /\ prog_reloctables p = prog_reloctables tp.
   
+
+Lemma reloc_prog_syneq_refl: forall t,
+    reloc_prog_syneq t t.
+Proof.
+  unfold reloc_prog_syneq.
+  intros. 
+  split. apply Permutation_refl.
+  intuition.
+  apply symbtable_syneq_refl.
+Qed.
+
+Lemma reloc_prog_syneq_symm: forall t1 t2,
+    reloc_prog_syneq t1 t2 -> reloc_prog_syneq t2 t1.
+Proof.
+  unfold reloc_prog_syneq.
+  intros. 
+  intuition.
+  apply symbtable_syneq_symm; auto.
+Qed.
+
+Lemma reloc_prog_syneq_trans: forall t1 t2 t3,
+    reloc_prog_syneq t1 t2 -> reloc_prog_syneq t2 t3 ->
+    reloc_prog_syneq t1 t3.
+Proof.
+  unfold reloc_prog_syneq.
+  intros. 
+  intuition.
+  eapply Permutation_trans; eauto.
+  eapply eq_trans; eauto.
+  eapply eq_trans; eauto.
+  eapply eq_trans; eauto.
+  eapply symbtable_syneq_trans; eauto.
+  eapply eq_trans; eauto.
+  eapply eq_trans; eauto.
+Qed.
